use option types in invariant

src/Examples/DistributedCtr/DistCtrImpl.v
@@ -9,55 +9,63 @@ Definition alloc : val := λ: "()",
   Pair (Pair (SOME "master") (SOME "backup")) "lk".
 
 Definition update_replica: val :=
-  λ: "replica1" "replica2",
+  λ: "replica1" "replica2" "lk",
+  acquire "lk";;
   match: "replica1" with
     SOME "r1" => 
-     match: "replica2" with
-       SOME "r2" => 
-            "r1" <- !"r1" + #1;;
-            "r2" <- !"r2" + #1
-       | NONE =>                       
-            "r1" <- !"r1" + #1;;
-            "r2" <- !"r1"
+    "r1" <- !"r1" + #1;;
+    match: "replica2" with
+      SOME "r2" => "r2" <- !"r2" + #1;;
+        release "lk";;
+        Pair (SOME "r1") (SOME "r2")
+    | NONE =>
+      let: "r2" := ref #0 in
+      "r2" <- !"r1";;
+      release "lk";;
+      Pair (SOME "r1") (SOME "r2")
      end
   | NONE =>
     match: "replica2" with
-       SOME "r2" => 
-            "r2" <- !"r2" + #1;;
-            "r1" <- !"r2"
-    | NONE => (* TODO should we just reallocate replica? *)
-       (Pair (Pair "replica1" "replica2") "ignore_lk") <- alloc #() 
+    SOME "r2" =>
+      let: "r1" := ref #0 in
+      "r2" <- !"r1"
+         "r2" <- !"r2" + #1;;
+        "r1" <- !"r2";;
+        release "lk";;
+        Pair (SOME "r1") (SOME "r2")
+    | NONE => "r1" <- ref #0;; "r2" <- ref #0
+        release "lk";;
+        Pair (SOME "r1") (SOME "r2")
     end
-  end;;
-  Pair "replica1" "replica2".
+  end.
 
 Definition get_replica: val :=
-  λ: "replica1" "replica2",
+  λ: "replica1" "replica2" "lk",
+  acquire "lk";;
   match: "replica1" with
-    SOME "r1" => !"r1"
+    SOME "r1" => "r" <- !"r1"
     | NONE => 
-     match: "replica2" with
-       SOME "r2" => 
-            !"r2"
-     | NONE => (* TODO should we just reallocate replica? *)
-       (Pair (Pair "replica1" "replica2") "ignore_lk") <- alloc #() 
+      match: "replica2" with
+        SOME "r2" => 
+        let: "r1" := ref #0 in
+        "r" <- !"r2";;
+        "r1" <- !"r2";;
+        release "lk";;
+        Pair (Pair (SOME "r1") (SOME "r2")) "r"
+       | NONE => "r1" <- ref #0;; "r2" <- ref #0
+        release "lk";;
+        Pair (Pair (SOME "r1") (SOME "r2")) "r"
      end
-  end;;
-  Pair "replica1" "replica2".
+  end.
 
+(* wrappers, not doing much right now. can we hide backup from the client? *)
 Definition update: val :=
   λ: "master" "backup" "lk",
-  acquire "lk";;
-  "replicas" <- update_replica "master" "backup";;
-  release "lk";;
-  "replicas".
+  update_replica "master" "backup".
 
 Definition get : val :=
   λ: "master" "backup" "lk",
-  acquire "lk";;
-  "replicas" <- get_replica "master" "backup";;
-  release "lk";;
-  Pair "replicas" "r".
+  get_replica "master" "backup".
 
 Section proof.
   Context `{!heapG Σ, !spawnG Σ, !lockG Σ, !inG Σ (authR (optionUR (exclR ZO)))}.
@@ -90,23 +98,25 @@ Section proof.
     done.
   Qed.
 
-  Definition update_inv (n1 n2 : Z) (mloc bloc : loc) (γ1 γ2 : gname) : iProp Σ :=
-    ⌜#n1 = #n2⌝
-    ∗ mloc ↦ #(n1)
-    ∗ bloc ↦ #(n2)
-    ∗ own γ1 (● (Excl' n1)) ∗ own γ2 (● (Excl' n2))%I.
-    (* we need these to tell the value of n1 and n2 *)
+  Definition update_inv (mloc bloc : option loc) (γ1 γ2 : gname) : iProp Σ := ∃ n : Z,
+      match mloc, bloc with
+      | Some m, Some b => m ↦ #(n) ∗ b ↦ #(n) ∗ own γ1 (● (Excl' n)) ∗ own γ2 (● (Excl' n))%I
+      | Some m, None => ∃ nloc, m ↦ #(n) ∗ nloc ↦ #(n) ∗ own γ1 (● (Excl' n)) ∗ own γ2 (● (Excl' n))%I
+      | None, Some b => ∃ nloc, nloc ↦ #(n) ∗ b ↦ #(n) ∗ own γ1 (● (Excl' n)) ∗ own γ2 (● (Excl' n))%I
+      | None, None => ∃ nloc1 nloc2, nloc1 ↦ #(n) ∗ nloc2 ↦ #(n) ∗ own γ1 (● (Excl' n)) ∗ own γ2 (● (Excl' n))%I
+      end.
+    (* we need these to tell the value of n *)
 
   (* Notes: loc = kind of like a Coq literal number, LitV (LitLoc loc) is an actual value in the language *)
 
-  Definition value_duplicated (n : Z) (r1 r2 : loc) (lk: val) : iProp Σ := ∃ (γ γ1 γ2 : gname), 
-    is_lock LockN γ lk (update_inv n n r1 r2 γ1 γ2) ∗ own γ1 (◯ (Excl' n)) ∗ own γ2 (◯ (Excl' n)).
+  Definition value_duplicated (n : Z) (r1 r2 : option loc) (lk: val) : iProp Σ := ∃ (γ γ1 γ2 : gname), 
+    is_lock LockN γ lk (update_inv r1 r2 γ1 γ2) ∗ own γ1 (◯ (Excl' n)) ∗ own γ2 (◯ (Excl' n)).
 
   Lemma alloc_spec : 
     {{{ True%I }}}
       alloc #()
     {{{ r1 r2 lk, RET PairV (PairV (SOMEV #r1) (SOMEV #r2)) lk;
-        value_duplicated 0 r1 r2 lk 
+        value_duplicated 0 (Some r1) (Some r2) lk
     }}}.
   Proof.
     iIntros (Φ) "_ HPost".
@@ -117,29 +127,114 @@ Section proof.
     wp_alloc master as "Hr1".
     wp_alloc backup as "Hr2"; wp_let.
  
-    wp_apply (newlock_spec LockN (update_inv 0 0 master backup γ1 γ2) with "[Hr1 Hr2 Hγ1● Hγ2●]").
+    wp_apply (newlock_spec LockN (update_inv (Some master) (Some backup) γ1 γ2) with "[Hr1 Hr2 Hγ1● Hγ2●]").
     unfold update_inv; iFrame; auto.
 
+    iExists 0. iFrame; auto.
     iIntros (lk γ) "HIsLk".
     wp_let.
     wp_pures.
-    iApply "HPost". unfold value_duplicated. 
+    iApply "HPost". unfold value_duplicated.
     iExists γ, γ1, γ2. iFrame; auto.
   Qed.
 
-  Lemma inc_spec : ∀ n r1 r2 lk, (*should γ be forall? *)
+  Lemma update_replica_some_spec : ∀ n master backup lk (r1 r2 : loc),
+      {{{ ⌜ (master = SOMEV #r1 ∧ backup = SOME #r2)
+          ∨ (master = SOMEV #r1 ∧ backup = NONEV)
+          ∨ (backup = SOMEV #r2 ∧ master = NONEV) ⌝
+          ∗ value_duplicated n r1 r2 lk
+
+      }}}
+      update_replica master backup lk
+      {{{ nr1 nr2, RET (SOMEV #nr1, SOMEV #nr2) ;
+          value_duplicated (n+1) nr1 nr2 lk
+      }}}.
+  Proof.
+    iIntros (n master backup lk r1 r2 ϕ) "Hvaldup Hϕ".
+    unfold update_replica.
+    iDestruct "Hvaldup" as ([[-> ->] | [[-> ->] | [-> ->]]]) "HInv";
+      iDestruct "HInv" as (γ γ1 γ2) "[#Hislk [Hγ1◯ Hγ2◯]]";
+      wp_pures;
+      wp_apply (acquire_spec with "[$Hislk]");
+      iIntros "(Hlked & HInv)";
+      wp_pures;
+      iDestruct "HInv" as (n') "(Hr1 & Hr2 & Hγ1● & Hγ2● )";
+        iDestruct (ghost_var_agree with "Hγ1● Hγ1◯") as %->;
+        iMod (ghost_var_update γ1 (n+1) with "Hγ1● Hγ1◯") as "[Hγ1● Hγ1◯]";
+        iMod (ghost_var_update γ2 (n+1) with "Hγ2● Hγ2◯") as "[Hγ2● Hγ2◯]".
+    - wp_load; wp_op; wp_store.
+      wp_load; wp_op; wp_store.
+      wp_apply (release_spec LockN γ lk (update_inv r1 r2 γ1 γ2) with "[- $Hlked Hγ1◯ Hγ2◯ Hϕ]").
+      iSplit; auto. unfold update_inv.
+      iExists (n + 1). iFrame; auto.
+      iIntros. wp_pures.
+      iApply "Hϕ".
+      iExists γ, γ1, γ2; iFrame; auto.
+    - wp_load; wp_op; wp_store.
+      wp_match.
+      wp_alloc r3 as "Hr3".
+      wp_let.
+      wp_load. wp_store.
+      wp_load. wp_store.
+      wp_load. 
+      wp_apply (release_spec LockN γ lk (update_inv r1 r2 γ1 γ2) with "[- $Hlked Hγ1◯ Hγ2◯ Hϕ]").
+      iSplit; auto. unfold update_inv.
+      iExists (n + 1). iFrame; auto.
+      iIntros. wp_pures.
+      iApply "Hϕ".
+      iExists γ, γ1, γ2; iFrame; auto.
+
+  Qed.
+ 
+  Lemma update_replica_none_spec : ∀ n master backup lk (r1 r2 : loc),
+      {{{ ⌜ master = NONE ∧ backup = SOMEV #r2 ⌝ ∗ value_duplicated n r1 r2 lk }}}
+      update_replica master backup lk
+      {{{ RET (SOMEV #r1, SOMEV #r2) ; value_duplicated (n+1) r1 r2 lk }}}.
+  Proof.
+    iIntros (n master backup lk r1 r2 ϕ) "Hvaldup Hϕ".
+    unfold update_replica.
+    wp_pures.
+    iDestruct "Hvaldup" as ([-> ->]) "HInv".
+    unfold value_duplicated in *.
+    iDestruct "HInv" as (γ γ1 γ2) "[#Hislk [Hγ1◯ Hγ2◯]]".
+
+    wp_apply (acquire_spec with "[$Hislk]").
+    iIntros "(Hlked & HInv)".
+    wp_pures.
+
+    iDestruct "HInv" as (n') "(Hr1 & Hr2 & Hγ1● & Hγ2● )".
+    iDestruct (ghost_var_agree with "Hγ1● Hγ1◯") as %->.
+    iMod (ghost_var_update γ1 (n+1) with "Hγ1● Hγ1◯") as "[Hγ1● Hγ1◯]".
+    iMod (ghost_var_update γ2 (n+1) with "Hγ2● Hγ2◯") as "[Hγ2● Hγ2◯]".
+
+    wp_load; wp_op; wp_store.
+    wp_load; wp_op; wp_store.
+    wp_apply (release_spec LockN γ lk (update_inv r1 r2 γ1 γ2) with "[- $Hlked Hγ1◯ Hγ2◯ Hϕ]").
+    iSplit; auto. unfold update_inv.
+    iExists (n + 1). iFrame; auto.
+
+    iIntros. wp_pures.
+    iApply "Hϕ".
+    iExists γ, γ1, γ2; iFrame; auto.
+  Qed.
+  
+  Lemma update_spec : ∀ n r1 r2 lk, (*should γ be forall? *)
     {{{ value_duplicated n r1 r2 lk }}}
-      inc (#r1, #r2) lk
+      update #r1 #r2 lk
     {{{ RET #() ; value_duplicated (n+1) r1 r2 lk }}}.
   Proof.
     iIntros (n r1 r2 lk ϕ) "Hvaldup Hϕ".
-    unfold inc.
+    unfold update.
     wp_pures.
     unfold value_duplicated in *.
     iDestruct "Hvaldup" as (γ γ1 γ2) "[Hislk [Hγ1◯ Hγ2◯]]".
     wp_apply (acquire_spec with "[Hislk]"). iApply "Hislk".
     iIntros "(Hlked & HInv)".
     wp_pures.
+    unfold update_replica. wp_pures.
+    induction r1.
+    induction r1.
+    iDestruct #r1 as "HR1". simpl.
     iDestruct "HInv" as "(_ & Hr1 & Hr2 & Hγ1● & Hγ2● )"; simpl in *.
     wp_apply (wp_par (λ _, own γ1 (◯ Excl' (n+1))) (λ _, own γ2 (◯ Excl' (n+1)))
                 with "[Hr1 Hγ1◯ Hγ1●] [Hr2 Hγ2◯ Hγ2●]").
@@ -151,7 +246,6 @@ Section proof.
       iNext.
       wp_pures.
       Check release_spec.
-      wp_apply ((release_spec LockN γ lk (parallel_inc_inv (n+1) (n+1) (r1, r2) γ1 γ2)) with "[Hlked Hγ1◯ Hγ2◯]").
 
       auto.
   Admitted.
